mechanization/theories/Core/Soundness/LogicalRelation/CoreLemmas.v
@@ -445,11 +445,11 @@ Proof.
 Qed.
 
 
-Lemma glu_sort_elem_core_sort' {P} (pred_P : PredicativeSig P) : forall s' s typ_rel el_rel,
+Lemma glu_sort_elem_core_sort' {P} (pred_P : PredicativeSig P) : forall s' s typ_rel exp_rel,
     Ax P s' s ->
     (typ_rel <∙> sort_glu_typ_pred pred_P s' s) ->
     (exp_rel <∙> sort_glu_exp_pred pred_P s' s) ->
-    {{ DG Sort@s' ∈ glu_sort_elem pred_P s ↘ typ_rel ↘ el_rel }}.
+    {{ DG Sort@s' ∈ glu_sort_elem pred_P s ↘ typ_rel ↘ exp_rel }}.
 Proof.
   intros.
   unshelve basic_glu_sort_elem_econstructor; mautosolve.
