mechanization/theories/Core/Soundness/SubstitutionCases.v
@@ -96,33 +96,46 @@ Qed.
 #[export]
 Hint Resolve glu_rel_sub_compose : mcpts.
 
-Lemma glu_rel_sub_extend {P} (pred_P : PredicativeSig P) (full_P : FullSig P) : forall {sts sts' Γ σ Δ M A s},
+Lemma glu_rel_sub_extend {P} (pred_P : PredicativeSig P) (full_P : FullSig P) : forall {sts sts' Γ σ Δ M A s s'},
     {{ ⟪ pred_P ⟫ Γ : sts ⊩s σ : Δ : sts' }} ->
-    {{ ⟪ pred_P ⟫ Δ : sts' ⊩ A : Sort@s }} ->
-    {{ ⟪ pred_P ⟫ Γ : sts ⊩ M : A[σ] }} ->
+    {{ ⟪ pred_P ⟫ Δ : sts' ⊩ A : Sort@s : s' }} ->
+    {{ ⟪ pred_P ⟫ Γ : sts ⊩ M : A[σ] : s }} ->
     {{ ⟪ pred_P ⟫ Γ : sts ⊩s (σ ,, M) : Δ , A : (s :: sts') }}.
 Proof.
   intros * Hσ HA HM.
   assert {{ Γ ⊢s σ : Δ }} by mauto 3.
   assert {{ Δ ⊢ A : Sort@s }} by mauto 3.
   assert {{ Γ ⊢ M : A[σ] }} by mauto 3.
-  assert (exists s', Ax P s s') as [s' ?]by (eapply full_P; mauto 2).
-  assert {{ ⟪ pred_P ⟫ Γ : sts ⊩ Sort@s : Sort@s' }} by mauto 3.
-  assert {{ Γ ⊢ Sort@s[σ] ≈ Sort@s }} by mauto 3.
-  assert {{ ⟪ pred_P ⟫ Γ : sts ⊩ A[σ] : Sort@s }} by mauto 3.
+  assert {{ Δ ⊢ Sort@s : Sort@s' }} by (eapply glu_rel_exp_typ_well_sorted; mauto 2).
+  assert (exists s'', {{ Δ ⊢ Sort@s'' ≈ Sort@s' }} /\ Ax P s s'') as [s'' []] by (eapply wf_exp_sort_sort; mauto 2).  
+  (* assert (exists s''', Ax P s'' s''') as [s'''] by (eapply full_P; mauto 2). *)
+  (* assert {{ ⟪ pred_P ⟫ Γ : sts ⊩ Sort@s : Sort@s'' : s''' }} by mauto 3. *)
+  (* assert {{ Γ ⊢ Sort@s[σ] ≈ Sort@s }} by mauto 3. *)
+  (* assert {{ ⟪ pred_P ⟫ Γ : sts ⊩ A[σ] : Sort@s : s' }} by mauto 3. *)
   destruct Hσ as [SbΓ [SbΔ]].
-  assert {{ ⟪ pred_P ⟫ Δ : sts' ⊩ Sort@s : Sort@s' }} by mauto 3.
   destruct_conjs.
-  invert_glu_rel_exp HA.
-  invert_glu_rel_exp HM.
+
+  destruct HA as [Sb []].
+  destruct HM as [Sb' []].
+  handle_functional_glu_ctx_env P.
+  
+  (* invert_glu_rel_exp HA. *)
+  (* invert_glu_rel_exp HM. *)
   do 2 eexists; repeat split; mauto.
   - econstructor; mauto 3; try reflexivity.
+    intros.
+    rewrite <- H14 in H5.
+    assert (glu_rel_exp_with_sub pred_P s' Δ0 A {{{ Sort@s }}} σ0 ρ) by mauto 2.
+    mauto 2.
+    
   - intros.
     handle_functional_glu_ctx_env P.
     destruct_glu_rel_sub_with_sub.
-    rewrite <- H17 in H8.
+    rewrite <- H14 in H8.
     destruct_glu_rel_sub_with_sub.
-    rewrite <- H18 in H14.
+    rewrite <- H15 in H5.
+    (* rewrite <- H14 in H12. *)
+    (* rewrite <- H14 in H16. *)
     destruct_glu_rel_exp_with_sub.
     simplify_evals.
     match_by_head (@glu_sort_elem P) ltac:(fun H => directed invert_glu_sort_elem H).
@@ -147,7 +160,7 @@ Proof.
       assert {{ Δ0 ⊢ A[Wk][(σ,,M)∘σ0] ≈ A[Wk∘((σ,,M)∘σ0)] : Sort@s }} as -> by (symmetry; mauto 3).
       assert {{ Δ0 ⊢ A[Wk∘((σ,,M)∘σ0)] ≈ A[σ∘σ0] : Sort@s }} as -> by mauto 3.
       assert {{ Δ0 ⊢ A[σ∘σ0] ≈ A[σ][σ0] : Sort@s }} by mauto 3.
-      rewrite -> H37.
+      rewrite -> H29.
       assert {{ Δ, A ⊢ #0 : A[Wk] }} by mauto 3.
       assert {{ Δ0 ⊢ #0[(σ,,M)∘σ0] ≈ #0[(σ∘σ0),,M[σ0]] : A[Wk][(σ,,M)∘σ0] }} by mauto 3.
       assert {{ Δ0 ⊢ #0[(σ,,M)∘σ0] ≈ #0[(σ∘σ0),,M[σ0]] : A[σ][σ0] }} as -> by mauto 4.
@@ -155,10 +168,8 @@ Proof.
       assert {{ Δ0 ⊢ #0[(σ∘σ0),,M[σ0]] ≈ M[σ0] : A[σ][σ0] }} as -> by (eapply wf_exp_eq_conv; mauto 4).
 
       eapply glu_sort_elem_exp_conv with (exp_rel := exp_rel); mauto 3.
-      rewrite <- H37.
-      eassumption.
+      eapply glu_sort_elem_trm_typ; mauto 2.
     + simpl.
-      eapply H17.
       eapply glu_ctx_env_sub_resp_sub_eq with (Sb := SbΔ) (σ := {{{ σ∘σ0 }}}); mauto 3.      
 Qed.
 
