mechanization/theories/Core/Soundness/TermStructureCases.v
@@ -5,20 +5,27 @@ From McPTS.Core.Semantic Require Import Realizability.
 From McPTS.Core.Soundness Require Import LogicalRelation.
 Import Domain_Notations.
 
-Lemma presup_glu_rel_exp {P} (pred_P : PredicativeSig P) (full_P : FullSig P) : forall {sts Γ M A},
-    {{ ⟪ pred_P ⟫ Γ : sts ⊩ M : A }} ->
-    {{ ⟪ pred_P ⟫ ⊩ Γ : sts }} /\ (exists s, {{ ⟪ pred_P ⟫ Γ : sts ⊩ A : Sort@s }}).
+Lemma presup_glu_rel_exp {P} (pred_P : PredicativeSig P) (full_P : FullSig P) : forall {sts s Γ M A},
+    {{ ⟪ pred_P ⟫ Γ : sts ⊩ M : A : s }} ->
+    {{ ⟪ pred_P ⟫ ⊩ Γ : sts }} /\ (exists s', {{ ⟪ pred_P ⟫ Γ : sts ⊩ A : Sort@s : s' }}).
 Proof.
-  intros * [? [? []]].
+  intros * [? []].
   split; [eexists; eassumption |].
+  assert (exists s', Ax P s s') as [s'] by (eapply full_P; mauto).
   do 2 eexists; intuition.
-  assert (exists s', Ax P x0 s') by (eapply full_P; mauto).
-  destruct_conjs.  
+  destruct_conjs.
+  destruct_glu_rel_exp_with_sub.
   eexists; mauto 4.
+  assert {{ Δ ⊢ Sort@s[σ] ≈ Sort@s }} by mauto 3.
+  assert {{ Δ ⊢ A[σ] : Sort@s }} by (eapply glu_sort_elem_trm_sort_lvl; mauto 2).
+  assert {{ Δ ⊢ A[σ] : Sort@s[σ] }} by mauto 3.
+  repeat split; mauto 3.
+  repeat eexists; mauto 2.
+  eapply glu_sort_elem_trm_typ; mauto 2.
 Qed.
 
-Lemma presup_ctx_glu_rel_exp {P} (pred_P : PredicativeSig P) (full_P : FullSig P) : forall {sts Γ M A},
-    {{ ⟪ pred_P ⟫ Γ : sts ⊩ M : A }} ->
+Lemma presup_ctx_glu_rel_exp {P} (pred_P : PredicativeSig P) (full_P : FullSig P) : forall {sts s Γ M A},
+    {{ ⟪ pred_P ⟫ Γ : sts ⊩ M : A : s }} ->
     {{ ⟪ pred_P ⟫ ⊩ Γ : sts }}.
 Proof.
   intros * []%presup_glu_rel_exp;
@@ -28,9 +35,9 @@ Qed.
 #[export]
 Hint Resolve presup_ctx_glu_rel_exp : mcpts.
 
-Lemma presup_typ_glu_rel_exp {P} (pred_P : PredicativeSig P) (full_P : FullSig P) : forall {sts Γ M A},
-    {{ ⟪ pred_P ⟫ Γ : sts ⊩ M : A }} ->
-    exists s, {{ ⟪ pred_P ⟫ Γ : sts ⊩ A : Sort@s }}.
+Lemma presup_typ_glu_rel_exp {P} (pred_P : PredicativeSig P) (full_P : FullSig P) : forall {sts s Γ M A},
+    {{ ⟪ pred_P ⟫ Γ : sts ⊩ M : A : s }} ->
+    exists s', {{ ⟪ pred_P ⟫ Γ : sts ⊩ A : Sort@s : s' }}.
 Proof.
   intros * []%presup_glu_rel_exp;
     eassumption.
@@ -42,57 +49,63 @@ Hint Resolve presup_typ_glu_rel_exp : mcpts.
 Lemma glu_rel_exp_vlookup {P} (pred_P : PredicativeSig P) (full_P : FullSig P) : forall {sts Γ x A},
     {{ #x : A ∈ Γ }} ->
     {{ ⟪ pred_P ⟫ ⊩ Γ : sts }} ->
-    {{ ⟪ pred_P ⟫ Γ : sts ⊩ #x : A }}.
+    exists s,
+    {{ ⟪ pred_P ⟫ Γ : sts ⊩ #x : A : s}}.
 Proof.
   intros * Hx.
   gen sts.
   induction Hx; intros * [Sb];
     match_by_head1 (@glu_ctx_env P) ltac:(fun H => invert_glu_ctx_env H).
-
   
   (* intros * [Sb] Hx. gen Sb. *)
   (* induction Hx; intros; *)
   (*   match_by_head1 (@glu_ctx_env P) ltac:(fun H => invert_glu_ctx_env H). *)
-  - eexists.
-    split; [econstructor |]; try reflexivity; mauto.
+  - exists s.
     eexists.
+    split; [econstructor |]; try reflexivity; mauto.
     intros.
     destruct_by_head (@cons_glu_sub_pred P).
     econstructor; mauto.
   - assert (glu_ctx_env pred_P {{{ sts, s }}} Sb {{{ Γ, B }}}) by (econstructor; mauto).
-    assert {{ ⟪ pred_P ⟫ Γ : sts ⊩ #n : A }} as Hn.
+    assert (exists s, {{ ⟪ pred_P ⟫ Γ : sts ⊩ #n : A : s}}) as [s' Hn].
     {
       eapply IHHx.
       econstructor; eauto.
     }
-    
-    assert (exists s, {{ Γ ⊢ A : Sort@s }}) as [s'] by (gen_presups; mauto 3).
-    invert_glu_rel_exp Hn.
-    rename x into k.
-    eexists.
+    assert (exists s, {{ Γ ⊢ A : Sort@s }}) as [s''] by (gen_presups; mauto 3).
+    inversion_clear Hn.
+    (* invert_glu_rel_exp Hn. *)
+    destruct_conjs.
+    handle_functional_glu_ctx_env P.
+    do 2 eexists.
     split.
     + econstructor; try reflexivity; mauto.
-      intros.
-      dependent destruction H3.
-      handle_functional_glu_ctx_env P.
-      eapply H5.
-      eassumption.
-    + eexists.
+   
+      (* intros. *)
+      (* dependent destruction H3. *)
+      (* handle_functional_glu_ctx_env P. *)
+      (* eapply H5. *)
+      (* eassumption. *)
+    + (* eexists. *)
       intros.
       destruct_by_head (@cons_glu_sub_pred P).
-      destruct_glu_rel_exp_with_sub.
+      rewrite <- H8 in H11.
+      destruct_glu_rel_exp_with_sub.      
       simplify_evals.
       rename a into b.
       rename a0 into a.
-      assert {{ Dom a ≈ a ∈ per_sort pred_P x0 }} as [] by mauto.
-      eapply mk_glu_rel_exp_with_sub''; intuition mauto.
+      assert {{ Dom a ≈ a ∈ per_sort pred_P s' }} as [] by mauto.      
+      eapply mk_glu_rel_exp_with_sub''; intuition mauto.      
       handle_functional_glu_sort_elem P.
       
-      
       assert {{ ⊢ Γ, B }} by mauto 3.
-      assert {{ Δ ⊢ A[Wk][σ] ≈ A[Wk∘σ] : Sort@s' }} by mauto.
-      assert {{ Γ ⊢ A : Sort@x0 }} by mauto.
-      assert {{ Δ ⊢ A[Wk][σ] ≈ A[Wk∘σ] : Sort@x0 }} as -> by mauto.
+      assert {{ Δ ⊢ A[Wk∘σ] : Sort@s' }} by (eapply glu_sort_elem_trm_sort_lvl; mauto 3).
+      assert {{ Δ ⊢ A[Wk][σ] ≈ A[Wk∘σ] : Sort@s' }} as ->.
+      {
+        assert (exists Δ0 K0, {{ Δ ⊢s Wk∘σ : Δ0 }} /\ {{ Δ0 ⊢ A : K0 }} /\ {{ Δ ⊢ K0[Wk∘σ] ≈ Sort@s' }}) as [Δ0 [K0 [? []]]] by mauto 2.
+        assert (exists Δ1, {{ Δ ⊢s σ : Δ1 }} /\ {{ Δ1 ⊢s Wk : Δ0 }}) as [Δ1 []] by mauto 2.
+        eapply wf_exp_eq_conv'; mauto 3.
+      }                                                                 
       assert {{ Γ ⊢ #n : A }} by mauto 4.
       assert {{ Γ, B ⊢ #n[Wk] : A[Wk] }} by mauto 3.
       assert {{ Γ, B ⊢ #n[Wk] ≈ #(S n) : A[Wk] }} by mauto 3.
@@ -104,84 +117,44 @@ Qed.
 #[export]
 Hint Resolve glu_rel_exp_vlookup : mcpts.
 
-Lemma glu_rel_exp_sub {P} (pred_P : PredicativeSig P) (full_P : FullSig P) : forall {sts Γ σ Δ sts' M A},
+Lemma glu_rel_exp_sub {P} (pred_P : PredicativeSig P) (full_P : FullSig P) : forall {sts Γ σ Δ sts' M A s},
     {{ ⟪ pred_P ⟫ Γ : sts ⊩s σ : Δ : sts' }} ->
-    {{ ⟪ pred_P ⟫ Δ : sts' ⊩ M : A }} ->
-    {{ ⟪ pred_P ⟫ Γ : sts ⊩ M[σ] : A[σ] }}.
-Proof.
+    {{ ⟪ pred_P ⟫ Δ : sts' ⊩ M : A : s }} ->
+    {{ ⟪ pred_P ⟫ Γ : sts ⊩ M[σ] : A[σ] : s }}.
+Proof .
   intros * Hσ HM.
   assert {{ Γ ⊢s σ : Δ }} by mauto 3.
   assert {{ Δ ⊢ M : A }} by mauto 3.
-  assert (exists s, {{ ⟪ pred_P ⟫ Δ : sts' ⊩ A : Sort@s }}) as [s] by mauto 3.
+  assert (exists s', {{ ⟪ pred_P ⟫ Δ : sts' ⊩ A : Sort@s : s' }}) as [s'] by mauto 3.
   destruct Hσ as [SbΓ [SbΔ]].
   destruct_conjs.
-  invert_glu_rel_exp HM.
+  inversion_clear HM as [? []].
+  (* invert_glu_rel_exp HM. *)
   assert {{ Δ ⊢ A : Sort@s }} by mauto 3.
   eexists; split; mauto.
-  eexists.
   intros Δ' τ ρ ?.
   destruct_glu_rel_sub_with_sub.
   handle_functional_glu_ctx_env P.
   rewrite <- H12 in H10.
   destruct_glu_rel_exp_with_sub.
-  assert {{ Dom a ≈ a ∈ per_sort pred_P x0 }} as [] by mauto.
+  assert {{ Dom a ≈ a ∈ per_sort pred_P s }} as [] by mauto.
   econstructor; mauto.
-  assert {{ Δ' ⊢s τ : Γ }} by mauto 3.
-  assert {{ Δ' ⊢ A[σ∘τ] : Sort@x0 }} by (eapply glu_sort_elem_trm_sort_lvl; mauto).
-  assert (exists Δ'' K, {{ Δ' ⊢s σ∘τ : Δ'' }} /\ {{ Δ'' ⊢ A : K }} /\ {{ Δ' ⊢ K[σ∘τ] ≈ Sort@x0 }}) by mauto.
-  destruct H18 as [Δ'' [? []]].
-  assert (exists Δ''', {{ Δ' ⊢s τ : Δ''' }} /\ {{ Δ''' ⊢s σ : Δ'' }}) by mauto.
-  destruct_conjs.
-  assert {{ Δ' ⊢ A[σ][τ] ≈ A[σ∘τ] : Sort@x0 }} as -> by (symmetry; mauto).
+
+  assert {{ Δ' ⊢ A[σ][τ] ≈ A[σ∘τ] : Sort@s }} as -> by (symmetry; mauto 4).
   assert {{ Δ' ⊢ M[σ][τ] ≈ M[σ∘τ] : A[σ∘τ] }} as ->; mauto 3.
+  symmetry; mauto 3.
 Qed.
 
 #[export]
 Hint Resolve glu_rel_exp_sub : mcpts.
 
 
-(* #[local] *)
-(* Lemma glu_rel_exp_conv' {P} (pred_P : PredicativeSig P) (full_P : FullSig P) : forall {sts Γ M A A' s}, *)
-(*     {{ ⟪ pred_P ⟫ Γ : sts ⊩ M : A }} -> *)
-(*     {{ Γ ⊢ A ≈ A' : Sort@s }} -> (** proof trick, will discharge. see the next lemma. *) *)
-(*     {{ Γ ⊢ A ≈ A' : Sort@s }} -> *)
-(*     {{ ⟪ pred_P ⟫ Γ : sts ⊩ M : A' }}. *)
-(* Proof. *)
-(*   intros * [? [? [k ?]]] [env_relΓ [? [? ?]]]%(completeness_fundamental_exp_eq P pred_P) ?. *)
-(*   econstructor; split; [eassumption |]. *)
-(*   exists (max i k); intros. *)
-(*   assert {{ Δ ⊢s σ : Γ }} by mauto 4. *)
-
-(*   destruct_glu_rel_exp_with_sub. *)
-(*   assert {{ Dom ρ ≈ ρ ∈ env_relΓ }} by (eapply glu_ctx_env_per_env; mauto). *)
-(*   (on_all_hyp: destruct_rel_by_assumption env_relΓ). *)
-(*   destruct_by_head rel_typ. *)
-(*   match_by_head eval_exp ltac:(fun H => directed dependent destruction H). *)
-(*   destruct_by_head rel_exp. *)
-(*   saturate_refl. *)
-(*   invert_per_univ_elems. *)
-(*   apply_equiv_left. *)
-(*   destruct_all. *)
-(*   handle_per_univ_elem_irrel. *)
-(*   assert (i <= max i k) by lia. *)
-(*   assert (k <= max i k) by lia. *)
-(*   assert {{ Δ ⊢ A'[σ] ≈ A[σ] : Type@(max i k) }} by mauto 4. *)
-(*   eapply mk_glu_rel_exp_with_sub''; intuition mauto using per_univ_elem_cumu_max_left, per_univ_elem_cumu_max_right. *)
-(*   bulky_rewrite. *)
-(*   eapply glu_univ_elem_exp_cumu_ge; try eassumption. *)
-(*   eapply glu_univ_elem_resp_per_univ; eauto. *)
-(*   symmetry. mauto. *)
-(* Qed. *)
-
-
-Lemma glu_rel_exp_conv {P} (pred_P : PredicativeSig P) (full_P : FullSig P) : forall {sts Γ M A A' s},
-    {{ ⟪ pred_P ⟫ Γ : sts ⊩ M : A }} ->
+Lemma glu_rel_exp_conv' {P} (pred_P : PredicativeSig P) (full_P : FullSig P) : forall {sts Γ M A A' s},
+    {{ ⟪ pred_P ⟫ Γ : sts ⊩ M : A : s }} ->
     {{ Γ ⊢ A ≈ A' : Sort@s }} ->
-    {{ ⟪ pred_P ⟫ Γ : sts ⊩ M : A' }}.
+    {{ ⟪ pred_P ⟫ Γ : sts ⊩ M : A' : s }}.
 Proof.
-  intros *.
-  
-  intros * [Sb [? [s' ?]]] HAA'.
+  intros * [Sb [?]] HAA'.
   assert {{ ⟪ pred_P ⟫ Γ ⊨u A ≈ A' : Sort@s }} as [env_relΓ [? ?]] by (eapply completeness_fundamental_exp_eq; mauto 2).
   
   assert (exists ρ ρ', initial_env Γ ρ /\ initial_env Γ ρ' /\ {{ Dom ρ ≈ ρ' ∈ env_relΓ }}) as [ρ [ρ']] by (eauto using per_ctx_then_per_env_initial_env).
@@ -202,9 +175,8 @@ Proof.
   rename m' into a'.
   
   eexists; split; [eauto |].
-  eexists.
   intros.
-  assert (glu_rel_exp_with_sub pred_P s' Δ M A σ ρ0) by mauto 2.
+  assert (glu_rel_exp_with_sub pred_P s Δ M A σ ρ0) by mauto 2.
   destruct H15.
   simplify_evals.
   handle_functional_glu_sort_elem P.
@@ -231,17 +203,92 @@ Proof.
   eapply glu_sort_elem_exp_conv with (a := a0) (a' := a0) (exp_rel := exp_rel0); mauto.
 
   assert (typ_rel0 Δ {{{ A [σ] }}}) by (eapply glu_sort_elem_trm_typ; mauto 2).
-
-  
-
-  
-  assert (exp_rel1 Δ {{{ A[σ] }}} {{{ M[σ] }}} m).
-  {
-    eapply glu_sort_elem_exp_conv with (exp_rel := exp_rel0); mauto 3.
-  }
-
-  by (eapply glu_sort_elem_exp_conv; mauto ).
-  
+  handle_functional_glu_sort_elem P.
+  eassumption.  
 Qed.
 
+
+
+(* Lemma glu_rel_exp_conv {P} (pred_P : PredicativeSig P) (full_P : FullSig P) : forall {sts Γ M A A' s}, *)
+(*     {{ ⟪ pred_P ⟫ Γ : sts ⊩ M : A : s }} -> *)
+(*     {{ Γ ⊢ A ≈ A' }} -> *)
+(*     {{ ⟪ pred_P ⟫ Γ : sts ⊩ M : A' : s }}. *)
+(* Proof. *)
+(*   intros * [Sb [?]] HAA'. *)
+(*   assert {{ ⟪ pred_P ⟫ Γ ⊨ A ≈ A' }} as [env_relΓ [? ?]] by (eapply completeness_fundamental_typ_eq; mauto 2). *)
+  
+(*   assert (exists ρ ρ', initial_env Γ ρ /\ initial_env Γ ρ' /\ {{ Dom ρ ≈ ρ' ∈ env_relΓ }}) as [ρ [ρ']] by (eauto using per_ctx_then_per_env_initial_env). *)
+(*   destruct_conjs. *)
+(*   assert (exists elem_rel : relation (domain P), *)
+(*              rel_typ_unsorted pred_P A ρ A' ρ' elem_rel) as [elem_rel] by mauto. *)
+  
+  
+(*   destruct_by_head (@rel_typ_unsorted P). *)
+(*   simplify_evals. *)
+  
+(*   assert {{ Γ ⊢s Id ® ρ ∈ Sb }} by (eapply initial_env_glu_rel_exp; mauto 2). *)
+(*   destruct_glu_rel_exp_with_sub. *)
+(*   simplify_evals. *)
+  
+(*   eexists; split; [eauto |]. *)
+(*   intros. *)
+(*   assert (glu_rel_exp_with_sub pred_P s Δ M A σ ρ0) by mauto 2. *)
+(*   destruct H14. *)
+(*   simplify_evals. *)
+(*   handle_functional_glu_sort_elem P. *)
+
+(*   assert (env_relΓ ρ0 ρ0) by (eapply glu_ctx_env_per_env; mauto 2). *)
+(*   assert (exists elem_rel0, rel_typ_unsorted pred_P A ρ0 A' ρ0 elem_rel0) as [elem_rel0] by mauto 2. *)
+(*   destruct_by_head (@rel_typ_unsorted P). *)
+(*   simplify_evals. *)
+(*   assert (per_typ_elem pred_P (per_sort pred_P s) d{{{ Sort@s }}} d{{{ Sort@s }}}) by (eapply per_typ_sort; reflexivity). *)
+(*   handle_per_typ_elem_irrel. *)
+(*   assert (per_sort pred_P s a0 a0) as [R] by mauto 3. *)
+(*   assert (per_sort_elem pred_P s elem_rel0 a0 a'0) by mauto 3. *)
+(*   assert (per_sort_elem pred_P s elem_rel0 a'0 a'0) by (transitivity a0; [symmetry |]; mauto 2). *)
+  
+(*   eapply mk_glu_rel_exp_with_sub''; mauto 3. *)
+(*   intros. *)
+(*   assert {{ Δ ⊢ A[σ] ≈ A'[σ] : Sort@s }} as <- by admit. *)
+
+(*   assert (glu_sort_elem pred_P s typ_rel1 exp_rel1 a0). *)
+(*   { *)
+(*     symmetry in H23. *)
+(*     eapply glu_sort_elem_resp_per_sort; mauto 3. *)
+(*   } *)
+(*   eapply glu_sort_elem_exp_conv with (a := a0) (a' := a0) (exp_rel := exp_rel0); mauto. *)
+
+(*   assert (typ_rel0 Δ {{{ A [σ] }}}) by (eapply glu_sort_elem_trm_typ; mauto 2). *)
+(*   handle_functional_glu_sort_elem P. *)
+(*   eassumption.   *)
+(* Qed. *)
+
+
+  
+(* Lemma glu_rel_exp_conv {P} (pred_P : PredicativeSig P) (full_P : FullSig P) : forall {sts s Γ M A A' }, *)
+(*     {{ ⟪ pred_P ⟫ Γ : sts ⊩ M : A : s }} -> *)
+(*     {{ Γ ⊢ A ≈ A' }} -> *)
+(*     {{ ⟪ pred_P ⟫ Γ : sts ⊩ M : A' : s }}. *)
+(* Proof. *)
+(*   intros. *)
+(*   enough {{ Γ ⊢ A ≈ A' : Sort@s }} by (eapply glu_rel_exp_conv'; mauto). *)
+(*   destruct H as [Sb [?]]. *)
+  
+(*   assert {{ ⟪ pred_P ⟫ Γ ⊨ A ≈ A' }} as [env_relΓ [? ?]] by (eapply completeness_fundamental_typ_eq; mauto 2).   *)
+(*   assert (exists ρ ρ', initial_env Γ ρ /\ initial_env Γ ρ' /\ {{ Dom ρ ≈ ρ' ∈ env_relΓ }}) as [ρ [ρ']] by (eauto using per_ctx_then_per_env_initial_env). *)
+(*   destruct_conjs. *)
+(*   assert (exists elem_rel : relation (domain P), rel_typ_unsorted pred_P A ρ A' ρ' elem_rel) by mauto 2. *)
+(*   destruct_conjs. *)
+(*   destruct_rel_typ_unsorted. *)
+  
+(*   assert {{ Γ ⊢s Id ® ρ ∈ Sb }} by (eapply initial_env_glu_rel_exp; mauto 2). *)
+(*   destruct_glu_rel_exp_with_sub. *)
+(*   simplify_evals. *)
+(*   assert (per_sort pred_P s a a) as [R] by mauto 2. *)
+(*   assert (per_sort_elem pred_P s H7 a a') by mauto 3. *)
+(*   assert (glu_sort_elem pred_P s typ_rel exp_rel a') by (eapply glu_sort_elem_resp_per_sort_elem with (typ_rel := typ_rel) (exp_rel := exp_rel); mauto 3). *)
+
+(*   assert {{ Γ ⊢ A[Id] ≈ A : Sort@s }} by mauto 4. *)
+(*   assert {{ Γ ⊢ A : Sort@s }} by mauto 3. *)
+  
   
